proved fundamental theorem of logical relation and adequacy of the denotational semantics wrt operational semantics up to a single remaining admit about substitution

theories/AlmostStlc/ContextEquiv.v
@@ -16,152 +16,325 @@ Require Export SemanticsFactsSeq.
 Require Export CallMrecFacts.
 Require Export SemanticsFactsSeq2.
 
-Definition context_equiv {t} (c1 c2 : comp t [] []) :=
-  forall b (r : bredex t [] + call_syn t []) (E : eval_context Nat [] r b) (n : nat),
-    eval_rel (subst_eval_context E c1) (val_const n) <-> eval_rel (subst_eval_context E c2) (val_const n).
-(*
-Equations type_inj (t : type) (v : denote_type t) : closed_value t
+(* not sure exactly how to define the contexts for contextual equivalence,
+   will need to keep track of variable context 
+   do I need stratification across
+
 *)
+(* seems like I might need 2 variable contexts one for  *)
+Inductive comp_context : vtype -> ctx -> mfix_ctx -> vtype -> ctx -> mfix_ctx -> Type :=
+  | ctx_hole {t Γ MR} : comp_context t Γ MR t Γ MR
+  | ctx_ret {t1 Γ1 MR1 t2 Γ2 MR2} (V : value_context t1 Γ1 t2 Γ2 MR2) : 
+    comp_context t1 Γ1 MR1 t2 Γ2 MR2
+  | ctx_let1 {Γ1 MR1 t1 t2 t3 Γ2 MR2} 
+             (C1 : comp_context t1 Γ1 MR1 t3 Γ2 MR2) (c2 : comp t2 (t1 :: Γ1) MR1) :
+    comp_context t2 Γ1 MR1 t3 Γ2 MR2
+  | ctx_let2 {Γ1 MR1 t1 t2 t3 Γ2 MR2} 
+             (c1 : comp t1 Γ1 MR1) (C2 : comp_context t2 (t1 :: Γ1) MR1 t3 Γ2 MR2) :
+    comp_context t2 Γ1 MR1 t3 Γ2 MR2
+  | ctx_match_nat1 {Γ1 MR1 t2 t3 Γ2 MR2} (Vn : value_context Nat Γ1 t3 Γ2 MR2)
+                   (cZ : comp t2 Γ1 MR1) (cS : comp t2 (Nat :: Γ1) MR1) : 
+    comp_context t2 Γ1 MR1 t3 Γ2 MR2
+  | ctx_match_nat2 {Γ1 MR1 t2 t3 Γ2 MR2} (vn : value Nat Γ1)
+                   (CZ : comp_context t2 Γ1 MR1 t3 Γ2 MR2) (cS : comp t2 (Nat :: Γ1) MR1) :
+    comp_context t2 Γ1 MR1 t3 Γ2 MR2
+  | ctx_match_nat3 {Γ1 MR1 t2 t3 Γ2 MR2} (vn : value Nat Γ1)
+                   (cZ : comp t2 Γ1 MR1) (CS : comp_context t2 (Nat :: Γ1) MR1 t3 Γ2 MR2) :
+    comp_context t2 Γ1 MR1 t3 Γ2 MR2
+  | ctx_succ {Γ1 MR1 t3 Γ2 MR2} (Vn : value_context Nat Γ1 t3 Γ2 MR2) : 
+    comp_context Nat Γ1 MR1 t3 Γ2 MR2
+  | ctx_match_list1 {t1 Γ1 MR1 t2 t3 Γ2 MR2} (VL : value_context (List t1) Γ1 t3 Γ2 MR2)
+                    (cnil : comp t2 Γ1 MR1) (ccons : comp t2 (t1 :: List t1 :: Γ1) MR1) : 
+    comp_context t2 Γ1 MR1 t3 Γ2 MR2
+  | ctx_match_list2 {t1 Γ1 MR1 t2 t3 Γ2 MR2} (vl : value (List t1) Γ1) 
+                    (Cnil : comp_context t2 Γ1 MR1 t3 Γ2 MR2) 
+                    (ccons : comp t2 (t1 :: List t1 :: Γ1) MR1) : 
+    comp_context t2 Γ1 MR1 t3 Γ2 MR2
+  | ctx_match_list3 {t1 Γ1 MR1 t2 t3 Γ2 MR2} (vl : value (List t1) Γ1)
+                    (cnil : comp t2 Γ1 MR1)
+                    (Ccons : comp_context t2 (t1 :: List t1 :: Γ1) MR1 t3 Γ2 MR2) :
+    comp_context t2 Γ1 MR1 t3 Γ2 MR2
+  | ctx_split1 {t1 t2 Γ1 MR1 t3 t4 Γ2 MR2} (Vp : value_context (Pair t1 t2) Γ1 t4 Γ2 MR2)
+               (cs : comp t3 (t1 :: t2 :: Γ1) MR1) : 
+    comp_context t3 Γ1 MR1 t4 Γ2 MR2
+  | ctx_split2 {t1 t2 Γ1 MR1 t3 t4 Γ2 MR2} (vp : value (Pair t1 t2) Γ1)
+               (Cs : comp_context t3 (t1 :: t2 :: Γ1) MR1 t4 Γ2 MR2) :
+    comp_context t3 Γ1 MR1 t4 Γ2 MR2
+  | ctx_app1 {t1 t2 Γ1 MR1 t3 Γ2 MR2} (Vf : value_context (Arrow t1 MR1 t2) Γ1 t3 Γ2 MR2)
+            (varg : value t1 Γ1) :
+    comp_context t2 Γ1 MR1 t3 Γ2 MR2
+  | ctx_app2 {t1 t2 Γ1 MR1 t3 Γ2 MR2} (vf : value (Arrow t1 MR1 t2) Γ1)
+             (Varg : value_context t1 Γ1 t3 Γ2 MR2) :
+    comp_context t2 Γ1 MR1 t3 Γ2 MR2
+  | ctx_call {t1 t2 Γ1 MR1 t3 Γ2 MR2 R}
+             (xR : var R MR1) (x : var (t1,t2) R)
+             (Vin : value_context t1 Γ1 t3 Γ2 MR2) : 
+    comp_context t2 Γ1 MR1 t3 Γ2 MR2
+  | ctx_lift {t1 Γ1 MR1 MR2 t2 Γ2 MR3}
+             (C : comp_context t1 Γ1 MR2 t2 Γ2 MR3) : 
+    comp_context t1 Γ1 (MR1 ++ MR2) t2 Γ2 MR3
+  | ctx_perm {t1 Γ1 MR1 MR2 t2 Γ2 MR3} (Hperm : perm MR1 MR2)
+             (C : comp_context t1 Γ1 MR1 t2 Γ2 MR3) : 
+    comp_context t1 Γ1 MR2 t2 Γ2 MR3
+  | ctx_mfix1 {t1 Γ1 R MR1 t2 Γ2 MR2}
+              (Bodies : bodies_context Γ1 MR1 R R t2 Γ2 MR2)
+              (c : comp t1 Γ1 (R :: MR1)) :
+    comp_context t1 Γ1 MR1 t2 Γ2 MR2
+  | ctx_mfix2 {t1 Γ1 R MR1 t2 Γ2 MR2}
+              (bodies : mfix_bodies Γ1 MR1 R R)
+              (C : comp_context t1 Γ1 (R :: MR1) t2 Γ2 MR2) : 
+    comp_context t1 Γ1 MR1 t2 Γ2 MR2
+with value_context : vtype -> ctx -> vtype -> ctx -> mfix_ctx -> Type :=
+  | ctx_cons1 {t1 Γ1 t2 Γ2 MR} 
+              (Vh : value_context t1 Γ1 t2 Γ2 MR)
+              (vt : value (List t1) Γ1) : 
+    value_context (List t1) Γ1 t2 Γ2 MR
+  | ctx_cons2 {t1 Γ1 t2 Γ2 MR}
+              (vh : value t1 Γ1)
+              (Vt : value_context (List t1) Γ1 t2 Γ2 MR) :
+    value_context (List t1) Γ1 t2 Γ2 MR
+  | ctx_pair1 {t1 t2 Γ1 t3 Γ2 MR}
+              (V1 : value_context t1 Γ1 t3 Γ2 MR)
+              (v2 : value t2 Γ1) :
+    value_context (Pair t1 t2) Γ1 t3 Γ2 MR
+  | ctx_pair2 {t1 t2 Γ1 t3 Γ2 MR}
+              (v1 : value t1 Γ1)
+              (V2 : value_context t2 Γ1 t3 Γ2 MR) : 
+    value_context (Pair t1 t2) Γ1 t3 Γ2 MR
+  | ctx_abs {t1 MR1 t2 Γ1 t3 Γ2 MR2}
+            (cbody : comp_context t2 (t1 :: Γ1) MR1 t3 Γ2 MR2) :
+      value_context (Arrow t1 MR1 t2) Γ1 t3 Γ2 MR2
+with bodies_context : ctx -> mfix_ctx -> call_frame -> call_frame -> vtype -> ctx -> mfix_ctx -> Type :=
+  | ctx_bodies_cons1 {t1 t2 Γ1 MR1 R1 R2 t3 Γ2 MR2}
+                     (Cbody : comp_context t2 (t1 :: Γ1) (R1 :: MR1) t3 Γ2 MR2)
+                     (bodies : mfix_bodies Γ1 MR1 R1 R2) :
+    bodies_context Γ1 MR1 R1 ((t1, t2) :: R2) t3 Γ2 MR2
+  | ctx_bodies_cons2 {t1 t2 Γ1 MR1 R1 R2 t3 Γ2 MR2}
+                     (cbody : comp t2 (t1 :: Γ1) (R1 :: MR1))
+                     (Bodies : bodies_context Γ1 MR1 R1 R2 t3 Γ2 MR2) :
+    bodies_context Γ1 MR1 R1 ((t1, t2) :: R2) t3 Γ2 MR2
+.
 
-(*
-Lemma types_equiv_eval_rel : 
-  forall t MR (v1 v2 : closed_value t) (c : comp t [] MR),
-    comp_equiv_rutt (denote_value v1 tt) (denote_value v2 tt) ->
-    comp_equiv_rutt (denote_comp c tt) (denote_value v1 tt) -> eval_rel c v2.
+Equations subst_comp_context {t1 Γ1 MR1 t2 Γ2 MR2}
+          (C : comp_context t1 Γ1 MR1 t2 Γ2 MR2) (c : comp t2 Γ2 MR2) : comp t1 Γ1 MR1 :=
+{
+  subst_comp_context ctx_hole c := c;
+  subst_comp_context (ctx_ret V) c := comp_ret (subst_value_context V c);
+  subst_comp_context (ctx_let1 C1 c2) c := comp_let (subst_comp_context C1 c) c2;
+  subst_comp_context (ctx_let2 c1 C2) c := comp_let c1 (subst_comp_context C2 c);
+  subst_comp_context (ctx_match_nat1 Vn cZ cS) c := 
+    comp_match_nat (subst_value_context Vn c) cZ cS;
+  subst_comp_context (ctx_match_nat2 vn CZ cS) c := 
+    comp_match_nat vn (subst_comp_context CZ c) cS;
+  subst_comp_context (ctx_match_nat3 vn cZ CS) c :=
+    comp_match_nat vn cZ (subst_comp_context CS c);
+  subst_comp_context (ctx_succ Vn) c := comp_succ (subst_value_context Vn c);
+  subst_comp_context (ctx_match_list1 Vl cnil ccons) c :=
+    comp_match_list (subst_value_context Vl c) cnil ccons;
+  subst_comp_context (ctx_match_list2 vl Cnil ccons) c :=
+    comp_match_list vl (subst_comp_context Cnil c) ccons;
+  subst_comp_context (ctx_match_list3 vl cnil Ccons) c :=
+    comp_match_list vl cnil (subst_comp_context Ccons c);
+  subst_comp_context (ctx_split1 Vp cs) c :=
+    comp_split (subst_value_context Vp c) cs;
+  subst_comp_context (ctx_split2 vp Cs) c :=
+    comp_split vp (subst_comp_context Cs c);
+  subst_comp_context (ctx_app1 Vf varg) c :=
+    comp_app (subst_value_context Vf c) varg;
+  subst_comp_context (ctx_app2 vf Varg) c :=
+    comp_app vf (subst_value_context Varg c);
+  subst_comp_context (ctx_call xR x Vin) c :=
+    comp_call xR x (subst_value_context Vin c);
+  subst_comp_context (ctx_lift C) c :=
+    comp_lift (subst_comp_context C c);
+  subst_comp_context (ctx_perm Hperm C) c :=
+    comp_perm Hperm (subst_comp_context C c);
+  subst_comp_context (ctx_mfix1 Bodies c) c0 :=
+    comp_mfix _ (subst_bodies_context Bodies c0) c;
+  subst_comp_context (ctx_mfix2 bodies C) c :=
+    comp_mfix _ bodies (subst_comp_context C c);
+}
+where subst_value_context {t1 Γ1 t2 Γ2 MR2}
+                   (V : value_context t1 Γ1 t2 Γ2 MR2) (c : comp t2 Γ2 MR2) : value t1 Γ1 :=
+{
+  subst_value_context (ctx_cons1 Vh vt) c := val_cons (subst_value_context Vh c) vt;
+  subst_value_context (ctx_cons2 vh Vt) c := val_cons vh (subst_value_context Vt c);
+  subst_value_context (ctx_pair1 V1 v2) c := val_pair (subst_value_context V1 c) v2;
+  subst_value_context (ctx_pair2 v1 V2) c := val_pair v1 (subst_value_context V2 c);
+  subst_value_context (ctx_abs Cbody) c := val_abs (subst_comp_context Cbody c);
+}
+where subst_bodies_context {Γ1 MR1 R1 R2 t2 Γ2 MR2}
+          (Bodies : bodies_context Γ1 MR1 R1 R2 t2 Γ2 MR2) 
+          (c : comp t2 Γ2 MR2) : mfix_bodies Γ1 MR1 R1 R2 :=
+{
+  subst_bodies_context (ctx_bodies_cons1 Cbody bodies) c :=
+    mfix_bodies_cons (subst_comp_context Cbody c) bodies;
+  subst_bodies_context (ctx_bodies_cons2 cbody Bodies) c :=
+    mfix_bodies_cons cbody (subst_bodies_context Bodies c);
+}.
 
-(* need to give this more thought *)
-Lemma equiv_value_eval_rel:
-  forall (v : nat) (c : comp Nat [] []),
-    comp_equiv_rutt (denote_comp c tt) (denote_value (val_const v) tt) -> eval_rel c (val_const v).
+Scheme comp_context_mind := Induction for comp_context Sort Prop
+  with value_context_mind := Induction for value_context Sort Prop
+  with bodies_context_mind := Induction for bodies_context Sort Prop.
+Combined Scheme context_mutind from comp_context_mind, value_context_mind, bodies_context_mind.
+
+Lemma subst_context_proper_mutind :
+  (forall t1 Γ1 MR1 t2 Γ2 MR2 (C : comp_context t1 Γ1 MR1 t2 Γ2 MR2)
+     (c1 c2 : comp t2 Γ2 MR2), 
+      comp_equiv (denote_comp c1) (denote_comp c2) -> 
+      comp_equiv 
+        (denote_comp (subst_comp_context C c1)) 
+        (denote_comp (subst_comp_context C c2))) /\
+  (forall t1 Γ1 t2 Γ2 MR2 (V : value_context t1 Γ1 t2 Γ2 MR2)
+     (c1 c2 : comp t2 Γ2 MR2),
+      comp_equiv (denote_comp c1) (denote_comp c2) ->
+      forall MR1, comp_equiv (MR := MR1)
+        (denote_value (subst_value_context V c1))
+        (denote_value (subst_value_context V c2))) /\
+  (forall Γ1 MR1 R1 R2 t2 Γ2 MR2 
+     (Bodies : bodies_context Γ1 MR1 R1 R2 t2 Γ2 MR2)
+     (c1 c2 : comp t2 Γ2 MR2),
+      comp_equiv (denote_comp c1) (denote_comp c2) ->
+      forall (arg1 arg2 : denote_call_frame R2) (hyps1 hyps2 : denote_ctx Γ1),
+        call_frame_pre_equiv R2 arg1 arg2 ->
+        ctx_equiv Γ1 hyps1 hyps2 ->
+        rutt (mfix_pre_equiv (R1 :: MR1)) (mfix_post_equiv (R1 :: MR1))
+             (call_frame_post_equiv R2 arg1 arg2)
+             (denote_bodies (subst_bodies_context Bodies c1) hyps1 arg1)
+             (denote_bodies (subst_bodies_context Bodies c2) hyps2 arg2)).
 Proof.
-  intros v c. revert v. dependent induction c; simp denote_comp.
-  - intros. dependent destruction v; try inversion x.
-    setoid_rewrite denote_value_equation_1 in H.
-Abort.
- *)
-Lemma subst_eval_context_proper:
-  forall (t1 t2 : vtype) MR1 MR2 (c1 c2 : comp t1 [] MR2) (b : bool) (r : bredex t1 MR2 + call_syn t1 MR2)
-    (E : eval_context t2 MR1 r b),
-    comp_equiv_rutt (denote_comp c1 tt) (denote_comp c2 tt) ->
-    comp_equiv_rutt (denote_comp (subst_eval_context E c1) tt)
-                    (denote_comp (subst_eval_context E c2) tt).
-Proof.
-  intros t1 t2 MR1 MR2 c1 c2 b r E.
-  revert c1 c2. dependent induction E; simp denote_comp; intros.
-  - simp subst_eval_context. simp denote_comp. eapply IHE in H; eauto.
-    eapply rutt_bind; eauto. intros. apply types_equiv_comp_refl.
+  apply context_mutind; intros; simp subst_comp_context.
+  - red. intros. simp denote_comp. eapply H; eauto.
+  - red. intros. simp denote_comp.
+    eapply rutt_bind; eauto. eapply H; eauto. intros.
+    eapply types_equiv_comp_refl. constructor; auto.
+  - red. intros. simp denote_comp.
+    eapply rutt_bind; eauto. eapply types_equiv_comp_refl; eauto.
+    intros. eapply H; eauto. constructor; eauto.
+  - red. intros. simp denote_comp.
+    eapply rutt_bind; eauto. eapply H; eauto. simp types_equiv.
+    intros. subst. destruct r2; eapply types_equiv_comp_refl; eauto.
+    constructor; eauto. simp types_equiv. auto.
+  - red. intros. simp denote_comp.
+    eapply rutt_bind; eauto. eapply types_equiv_value_refl; auto.
+    simp types_equiv. intros. subst. destruct r2.
+    eapply H; eauto. eapply types_equiv_comp_refl; auto. constructor; auto.
+    simp types_equiv. auto.
+  - red. intros. simp denote_comp.
+    eapply rutt_bind; eauto. eapply types_equiv_value_refl; auto.
+    simp types_equiv. intros. subst. destruct r2.
+    eapply types_equiv_comp_refl; auto. eapply H; auto.
+    constructor; auto. simp types_equiv. auto.
+  - red. intros. simp denote_comp.
+    eapply rutt_bind; eauto. eapply H; eauto.
+    simp types_equiv. intros. subst. apply rutt_Ret. auto.
+  - red. intros. simp denote_comp.
+    eapply rutt_bind; eauto.
+    eapply H; eauto. simp types_equiv. intros.
+    dependent destruction H2. eapply types_equiv_comp_refl; eauto.
+    eapply types_equiv_comp_refl; eauto. constructor; auto. constructor; auto.
+  - red. intros. simp denote_comp.
+    eapply rutt_bind; eauto. eapply types_equiv_value_refl; eauto.
+    simp types_equiv. intros. dependent destruction H2.
+    eapply H; eauto. apply types_equiv_comp_refl; auto.
     repeat constructor; auto.
-  - simp subst_eval_context. simp denote_comp.
-    eapply IHE in H; eauto. 
-    eapply interp_mrec_rutt with 
-        (RPreInv := call_frame_pre_equiv _)
-        (RPostInv := call_frame_post_equiv _); intros; eauto.
-    eapply types_equiv_mfix_bodies_refl. constructor. auto.
-  - simp subst_eval_context. simp denote_comp.
-    eapply IHE in H as IHE'; eauto. eapply mapE_rutt.
-    eapply rutt_mon; try eapply IHE'; auto.
-        apply mfix_pre_equiv_perm_handler.
-        apply mfix_post_equiv_perm_handler.
-  - simp subst_eval_context. simp denote_comp.
-    eapply IHE in H as IHE'; eauto. eapply mapE_rutt.
-    eapply rutt_mon; try eapply IHE'; auto.
-        apply mfix_pre_equiv_lift_handler.
-        apply mfix_post_equiv_lift_handler.
+  - red. intros. simp denote_comp.
+    eapply rutt_bind; eauto. eapply types_equiv_value_refl; eauto.
+    simp types_equiv. intros. dependent destruction H2.
+    eapply types_equiv_comp_refl; eauto.
+    apply H; auto. repeat constructor; auto.
+  - red. intros. simp denote_comp.
+    eapply rutt_bind; eauto. eapply H; eauto.
+    simp types_equiv. intros. dependent destruction H2.
+    destruct r1. destruct r2. eapply types_equiv_comp_refl; eauto.
+    repeat constructor; auto.
+  - red. intros. simp denote_comp.
+    eapply rutt_bind; eauto. eapply types_equiv_value_refl; eauto.
+    simp types_equiv. intros. dependent destruction H2.
+    destruct r1. destruct r2. eapply H; auto.
+    repeat constructor; auto.
+  - red. intros. simp denote_comp.
+    eapply rutt_bind; eauto. eapply H; auto.
+    intros. simp types_equiv in H2. eapply rutt_bind.
+    eapply types_equiv_value_refl; eauto. intros.
+    setoid_rewrite tau_eutt. eauto.
+  - red. intros. simp denote_comp.
+    eapply rutt_bind; eauto. eapply types_equiv_value_refl; eauto.
+    simp types_equiv. intros. eapply rutt_bind.
+    eapply H; auto. intros. setoid_rewrite tau_eutt. eauto.
+  - red. intros. simp denote_comp.
+    eapply rutt_bind; eauto. eapply H; auto.
+    intros. unfold call_term.
+    destruct (call_mrec x xR r1) as [ca1 f1] eqn : Heq1.
+    destruct (call_mrec x xR r2) as [ca2 f2] eqn : Heq2. 
+    setoid_rewrite bind_trigger. apply rutt_Vis.
+    eapply mfix_pre_call_mrec; eauto. intros.
+    apply rutt_Ret. eapply mfix_post_equiv_types_equiv; eauto.
+  - red. intros. simp denote_comp.
+    eapply mapE_rutt. eapply rutt_mon; try eapply H; eauto.
+    intros. eapply mfix_pre_equiv_lift_handler; eauto.
+    intros. eapply mfix_post_equiv_lift_handler; eauto.
+  - red. intros. simp denote_comp.
+    eapply mapE_rutt. eapply rutt_mon; try eapply H; eauto.
+    intros. eapply mfix_pre_equiv_perm_handler; eauto.
+    intros. eapply mfix_post_equiv_perm_handler; eauto.
+  - red. intros. simp denote_comp.
+    eapply interp_mrec_rutt
+     with (RPreInv := call_frame_pre_equiv R)
+          (RPostInv := call_frame_post_equiv R).
+    intros. eapply H; eauto.
+    eapply types_equiv_comp_refl with (c := c); auto.
+  - red. intros. simp denote_comp.
+    eapply interp_mrec_rutt
+     with (RPreInv := call_frame_pre_equiv R)
+          (RPostInv := call_frame_post_equiv R).
+    intros. eapply types_equiv_mfix_bodies_refl; eauto.
+    eapply H; auto.
+  - red. intros. simp denote_comp.
+    eapply rutt_bind. eapply H; eauto. intros.
+    eapply rutt_bind. eapply types_equiv_value_refl; auto.
+    simp types_equiv. intros.
+    apply rutt_Ret. constructor; auto.
+  - red. intros. simp denote_comp.
+    eapply rutt_bind. eapply types_equiv_value_refl; auto.
+    intros. eapply rutt_bind. eapply H; eauto.
+    intros. apply rutt_Ret. constructor; auto.
+  - red. intros. simp denote_comp.
+    eapply rutt_bind. eapply H; eauto. intros.
+    eapply rutt_bind. eapply types_equiv_value_refl; auto.
+    simp types_equiv. intros.
+    apply rutt_Ret. constructor; auto.
+  - red. intros. simp denote_comp.
+    eapply rutt_bind. eapply types_equiv_value_refl; auto.
+    intros. eapply rutt_bind. eapply H; eauto.
+    intros. apply rutt_Ret. constructor; auto.
+  - red. intros. simp denote_comp.
+    apply rutt_Ret. simp types_equiv. intros. eapply H; eauto.
+    constructor; auto.
+  - simp types_equiv in H1. dependent destruction H1; simp denote_comp.
+    + eapply rutt_mon; try eapply H; eauto. simp types_equiv. intros.
+      constructor. auto. constructor; auto.
+    + eapply types_equiv_mfix_bodies_refl with (bodies := bodies) in H2; eauto. 
+      specialize (H2 H1). eapply rutt_mon; try eapply H2; eauto.
+      intros. simp types_equiv. constructor. auto.
+  - simp types_equiv in H1. dependent destruction H1; simp denote_comp.
+    + eapply rutt_mon; try eapply types_equiv_comp_refl; eauto. simp types_equiv. intros.
+      constructor. auto. constructor; auto.
+    + eapply rutt_mon; try eapply H; eauto.
+      simp types_equiv. intros; constructor; auto.
 Qed.
 
-
-
-
-
-(* this doesn't feel quite right *)
-Lemma comp_equiv_value_eval:
-  forall (t : vtype) (MR : mfix_ctx) (c : comp t [] MR) (v : closed_value t),
-    comp_equiv_rutt (denote_comp c tt) (denote_value v tt) -> 
-    exists (v' : closed_value t), comp_equiv_rutt (MR := MR) (denote_value v tt) (denote_value v' tt) -> eval_rel c v'.
+Lemma subst_comp_context_proper t1 Γ1 MR1 t2 Γ2 MR2 (C : comp_context t1 Γ1 MR1 t2 Γ2 MR2)
+     (c1 c2 : comp t2 Γ2 MR2) :  
+      comp_equiv (denote_comp c1) (denote_comp c2) -> 
+      comp_equiv 
+        (denote_comp (subst_comp_context C c1)) 
+        (denote_comp (subst_comp_context C c2)).
 Proof.
-  intros t MR c v Hv. dependent induction c.
-  - intros. exists v. intros. constructor. cbv. simp observe. auto.
-  - intros. 
-    (* might need to be more general and might need a different ind hyp,
-       the problem is I don't know how to generalize this further because taking
-       a step only seems to make sense for closed terms,
-       could be more general if I went relational, but I want
-       to try to find a different solution before biting that bullet
+  destruct subst_context_proper_mutind. eauto.
+Qed.
 
-       I could possibly generalize by putting in an assumption that
-       hypotheses all have corresponding values (stronger condition than in logical relation)
-
-       could rely on folding substitution multiple times
-
-       or could maybe generalize 
-
-     *)
-    specialize (IHc1 c1 eq_refl JMeq_refl).
-Abort.
-
-
-(* do we need lem, I think no because we have evidence tha denote_comp c is ret *)
-Theorem adequacy : forall t (c1 c2 : comp t [] []),
-    comp_equiv_rutt (denote_comp c1 tt) (denote_comp c2 tt) ->
-    context_equiv c1 c2.
-Proof.
-  intros t c1 c2 Hden b r E v.
-  assert (Hden' : comp_equiv_rutt (denote_comp (subst_eval_context E c1) tt)
-                                  (denote_comp (subst_eval_context E c2) tt)).
-  apply subst_eval_context_proper. auto.
-  remember (subst_eval_context E c1) as c1'.
-  remember (subst_eval_context E c2) as c2'.
-  clear Heqc1' Heqc2'.
-  split; intros Hc1.
-  - generalize dependent c2'. clear - Hden Hc1.
-    induction Hc1.
-    + intros. apply IHHc1. apply step_stable in H.
-      symmetry in H. etransitivity; eauto.
-    + intros. apply step_stable2 in H.
-      assert (Hv : comp_equiv_rutt (denote_comp c2' tt) (denote_value v0 tt) ).
-      etransitivity; eauto. symmetry. auto. clear - Hv.
-      red in Hv. setoid_rewrite types_equiv_equation_1 in Hv.
-      (* my concern is that the inductive hyp may require *) 
-      assert ((exists v', eval_rel c2' v') \/ ~ exists v', eval_rel c2' v').
-      admit. (* classical reasoning *)
-      destruct H.
-      * destruct H as [v' Hv']. 
-        red in v0, v'. dependent destruction v0; try inversion x.
-        dependent destruction v'; try inversion x.
-        enough (n = n0); subst; auto.
-        apply eval_stable in Hv'.
-        rewrite denote_value_equation_1 in Hv, Hv'.
-        assert (comp_equiv_rutt (t := Nat) (MR := []) (ret n) (ret n0)).
-        etransitivity; eauto. symmetry. auto.
-        apply rutt_inv_Ret in H. simp types_equiv in H.
-      * red in v0. dependent destruction v0; try inversion x.
-        rewrite denote_value_equation_1 in Hv.
-        exfalso. red in H.
-        (* this seems like the best hope *)
-        enough ((denote_comp c2' tt) ≈ EnTree.spin ).
-        red in Hv. rewrite H0 in Hv. admit.
-        eapply H. exists (val_const n).
-        apply eval_stable in H.
-
-(* transform H into evidence  that denote_comp c2' is spin,
-           this contradicts Hv
-         *) admit.
-      (* maybe need that if denote_comp c tt = ret v then eval
-         i get the feeling this might be easier to do with 
-         relational, maybe also might be easier with lem 
-
-         show the connect
-
-       *)
-
-        
-      (* may be its own lemma *)
-      constructor 2.
-      apply  observe_inr_comp_ret.
-      (* need to think this through carefully *)
-      admit.
-    remember ()
-    generalize dependent c2.  dependent induction Hc1; intros.
-    + specialize (IHHc1 b t c1 c2 Hden r E).
-    
-(* will need a logical relation for proving the last piece of adequacy, *)
+Definition context_equiv {t Γ MR} (c1 c2 : comp t Γ MR) : Prop :=
+  forall (C : comp_context Nat [] [] t Γ MR) (n : nat),
+    eval_rel (subst_comp_context C c1) (val_const n) <->
+      eval_rel (subst_comp_context C c2) (val_const n).
