theories/AlmostStlc/Adequacy.v
@@ -1,4 +1,3 @@
-
 Require Export TypedVar.
 Require Export SyntaxSeq.
 Require Export SmallStepSeq.
@@ -22,221 +21,77 @@ Require Import Coq.Classes.Morphisms.
 Require Export ClosingSubst.
 Require Export LogicalApprox.
 Require Export Compatibility.
+Require Export RuttFacts.
+Require Export ContextEquiv.
 
 (* do compatibility lemmas first, one compatibility for each typing derivation  *)
 
-Theorem fundamental_theorem_adequacy :
-  forall n,
-  (forall (t : vtype) (Γ : ctx) (MR : mfix_ctx) (c : comp t Γ MR) (ρ : closing_subst Γ) (hyps : denote_ctx Γ), 
-      closing_subst_approx n Γ hyps ρ-> approx_comp n approx_val (denote_comp c hyps)  (close_comp Γ ρ c) 
-  ) /\
-  (forall (t : vtype) (Γ : ctx) (v : value t Γ) (ρ : closing_subst Γ) (hyps : denote_ctx Γ), 
-      closing_subst_approx n Γ hyps ρ -> forall vv MR, comp_equiv_rutt (ret vv) (denote_value (MR := MR) v hyps) -> approx_val n t vv (close_value Γ ρ v)) /\
-  (forall (Γ : ctx) (MR : mfix_ctx) (R1 R2 : call_frame) (bodies : mfix_bodies Γ MR R1 R2) (ρ : closing_subst Γ) (hyps : denote_ctx Γ), 
-      closing_subst_approx n Γ hyps ρ -> 
-      log_rel_bodies_step n (denote_bodies bodies hyps) (close_bodies Γ ρ bodies)).
+Theorem fundamental_theorem_adequacy_mutind : 
+  (forall t Γ MR (c : comp t Γ MR), comp_rel (denote_comp c) c) /\
+  (forall t Γ (v : value t Γ) MR, val_rel (MR := MR) (denote_value v) v) /\
+  (forall Γ MR R1 R2 (bodies : mfix_bodies Γ MR R1 R2), bodies_rel (denote_bodies bodies) bodies).
 Proof.
-  intros n. induction n as [ n IHn ] using (well_founded_induction lt_wf).
-  (*
-  destruct n.
-  {
-    split. 2 : split.
-    all : intros.
-    - constructor. intros. lia.
-    - simp approx_val. auto.
-    - simp log_rel_bodies_step.
-      dependent induction bodies.
-      simp log_rel_bodies_step. simp close_bodies. admit.
-      admit. (* this should hold, but the relation is in a very sketchy state right now,
-                so don't bother*)
-  } *) (*
-  assert (IHnc : forall y, y < n -> 
-          (forall (t : vtype) (Γ : ctx) (MR : mfix_ctx) (c : comp t Γ MR) (ρ : closing_subst Γ)
-           (hyps : denote_ctx Γ),
-         closing_subst_approx y Γ hyps ρ ->
-         approx_comp y approx_val (denote_comp c hyps) (close_comp Γ ρ c) )).
-  { intros m Hm. apply IHn in Hm. tauto. }
-  assert (IHnv : forall y, y < n -> 
-         (forall (t : vtype) (Γ : ctx) (v : value t Γ) (ρ : closing_subst Γ) (hyps : denote_ctx Γ),
-          closing_subst_approx y Γ hyps ρ ->
-         forall (vv : denote_type t) (MR : mfix_ctx),
-         comp_equiv_rutt (MR := MR) (denote_value v hyps) (ret vv) -> approx_val y t vv (close_value Γ ρ v))).
-  { intros m Hm. apply IHn in Hm. intros. eapply Hm; eauto. symmetry. apply H0. }
-  assert (IHnbodies : forall y, y < n -> 
-         (forall (Γ : ctx) (MR : mfix_ctx) (R1 R2 : call_frame) (bodies : mfix_bodies Γ MR R1 R2)
-           (ρ : closing_subst Γ) (hyps : denote_ctx Γ),
-         closing_subst_approx y Γ hyps ρ ->
-         log_rel_bodies_step y (denote_bodies bodies hyps) (close_bodies Γ ρ bodies))).
-  { intros m Hm. apply IHn in Hm. tauto. }
-  clear IHn.
-  apply comp_value_mutind; intros; auto.
-  - rewrite denote_value_equation_1 in H0. apply rutt_inv_Ret in H0.
-    simp types_equiv in H0. subst.
-    (* show that close_value (val_const) is val_const *) admit.
- - rewrite denote_value_equation_2 in H0. apply rutt_inv_Ret in H0.
-   inversion H0. subst.
-   (*show close_value val_nil is val_nil *) admit.
- - rewrite denote_value_equation_3 in H2. 
-   admit.
- - rewrite denote_value_equation_4 in H2. destruct vv as [vv1 vv2].
-   (* wts close_value commutes with val_pair *) admit.
- - rewrite denote_value_equation_5 in H1. apply rutt_inv_Ret in H1.
-   rename vv into f.
-   rewrite close_value_abs.
-   (* there is another reasoning principle I need here *)
-   destruct n; simp approx_val; auto. intros vv v m' Hm' Hvv Hv.
-   apply lower_approx_comp_aux3; auto.  
-   specialize (IHnc m' Hm'). Locate close_comp_app. Locate close_comp. (* do these functions need to be separately defined does one subsume the other? *)
-   assert (subst_comp_cons (close_comp_app (Γ1 := [t1]) ρ cbody) v = close_comp (t1 :: Γ) (v,ρ) cbody ).
-   (* admitted lemma *)
-   rewrite subst_comp_const_close. simp close_comp. auto.
-   rewrite H2.
-   simp types_equiv in H1.   
-   specialize (H1 vv vv Hvv).
-   rewrite H1.
-   eapply IHnc. constructor; auto.
-   eapply lower_closing_subst_approx; eauto.
- - rewrite denote_value_equation_6 in H0.
-   apply rutt_inv_Ret in H0.
-   clear - H H0. rewrite H0. clear H0. dependent induction x.
-   + destruct ρ as [v ρ]. destruct hyps as [vv0 hyps]. dependent destruction H. simp index_ctx.
-     simp close_value. unfold subst_value_cons. simp subst_value. admit.
-   + destruct ρ as [v ρ]. destruct hyps as [vv0 hyps]. simp index_ctx.
-     (* should just write a lemma about close_value *)
-     simp close_value. (* subst_value_cons (var (VarS x)) x = var x*)
-     admit.
-   (* this makes sense but lets put it in a separate lemma 
-   dependent induction H. inversion x.
-   dependent destruction x.
-   + simp close_value. unfold subst_value_cons. rewrite subst_value_equation_6. simp subst_var.
-     simp index_ctx in H1. rewrite H1. admit.
-   + simp close_value. simp index_ctx in H1. rewrite H1. unfold subst_value_cons. simp subst_value.
+  apply comp_value_mutind; intros.
+  - apply const_compat.
+  - apply nil_compat.
+  - apply cons_compat; auto.
+  - apply pair_compat; auto.
+  - apply abs_compat; auto.
+  - apply var_compat; auto.
+  - specialize (H MR). apply ret_compat in H. eauto.
+  - eapply let_compat in H; eauto. unfold comp_bind in H. eauto.
+  - eapply match_nat_compat in H0; eauto. eauto.
+  - specialize (H MR). eapply succ_compat in H. eauto.
+  - eapply match_list_compat in H0; eauto. eauto.
+  - eapply split_compat in H0; eauto. eauto.
+  - specialize (H0 MR). eapply app_compat in H0; eauto.
+    eauto.
+  - specialize (H MR). eapply call_compat with (xR := xR) (x := x) in H; eauto.
+  - eapply mfix_compat in H; eauto. eauto.
+  - eapply lift_compat with (MR1 := MR1) in H; eauto.
+  - eapply perm_compat with (Hperm := Hperm) in H; eauto.
+  - apply mfix_bodies_nil_compat.
+  - apply mfix_bodies_cons_compat; auto.
+Qed.
 
-   dependent induction x.
-   + destruct ρ as [vv0 ρ]. simp close_value. rename l into Γ. (* need to induct on Γ*) admit.
-   + destruct  ρ as [vv0 ρ]. simp close_value.
 
-   admit. admit. *)
- - rewrite denote_comp_equation_1. constructor. intros. split.
-   + intros. exists (close_value Γ ρ v). symmetry in H2. eapply H in H0; eauto.
-     split. admit. (* prove close_comp commutes with comp_ret *)
-     eapply lower_approx_val; try apply H0; eauto. lia.
-   + intros. specialize denote_value_terminates with (v := v) (hyps := hyps) as [ vv Hterm].
-     red in H2. rewrite Hterm in H2.
-     (* prove call_term has a vis at the head, then derive contradiction from H2 *)
-     admit.
- - rewrite denote_comp_equation_2. apply H in H1 as Hc1.
-   rename H0 into Hc2.  inversion Hc1. subst. 
-   constructor. intros Hn. specialize (H0 Hn) as [Hretc1 Hstuckc1]. split.
-   + intros vv3 Hvv3. 
-     assert (exists vv1, comp_equiv_rutt (denote_comp c1 hyps) (ret vv1) ).
-     admit. 
-     destruct H0 as [vv1 Hvv1]. 
-     specialize (Hretc1 vv1 Hvv1) as [v1 [Hv11 Hv12]].
-     assert (HΓ : closing_subst_approx (n - 1) (t1 :: Γ) (vv1,hyps) (v1, ρ)).
-     { constructor. auto. eapply lower_closing_subst_approx; eauto. lia. }
-     eapply IHnc with (c := c2) in HΓ as Hc2'.
-     inversion Hc2'. subst. rename H0 into Hpredn. 
-     assert (n = 1 \/ n - 1 > 0). lia.
-     destruct H0.
-     * subst. cbn in *.
-       (* think this through carefully, there seems to be a problem if n = 1*) admit.
-     * destruct (Hpredn H0) as [Hretc2 Hstuckc2]. clear Hpredn.
-
-     (* problem with rewriting with comp_equiv_rutt and bind rewrite Hvv1 in Hvv3. *)
-     
-     
-        (* can use Hvv3 to prove that c1 and c2 evaluate to rets
-           then use Hretc1 to create a closing subst
-         *)
-    (* destruct H2 as [Hc11 Hc12].
-   constructor. admit. split.
-   + intros.
-     assert (Hvv1 : exists vv1, comp_equiv_rutt (denote_comp c1 hyps) (ret vv1) ).
-     admit.
-     destruct Hvv1 as [vv1 Hvv1]. apply Hc11 in Hvv1 as Hvv1'.
-     destruct Hvv1' as [v1 [Hv11 Hv12]]. clear Hc12.
-     assert (Hρ :  closing_subst_approx (S n) (t1 :: Γ) (v1, ρ) (vv1, hyps)).
-     constructor; auto.
-     specialize (Hc2 (v1, ρ) (vv1, hyps) Hρ). inversion Hc2.
-     subst. destruct H4 as [Hc21 Hc22]. clear Hc22.
-     assert (Hvv2 : exists vv2, comp_equiv_rutt (denote_comp c2 (vv1,hyps)) (ret vv2)).
-     admit.
-     destruct Hvv2 as [vv2 Hvv2].
-     apply Hc21 in Hvv2 as Hvv2'. destruct Hvv2' as [v2 [Hv21 Hv22] ].
-     assert (types_equiv _ vv2 vv).
-     (* from H2 and the equivalence to rets *) admit.
-     exists v2.
-     split.
-     (* congruence rules I will need to make + Hvv1 and Hv11 Hv21 *)
-     admit.
-     (* rewrite acording to the types_equiv in H4 *)
-     admit.
-   + intros.
-     (* will need itree rule that either denote_comp c1 as a vis, or 
-        denote_comp c1 is a ret and denote_comp c2 is a vis
-      *) admit.
- - rewrite denote_comp_equation_3. (*comp_match_nat and bind *)
-   admit.
- - rewrite denote_comp_equation_4. (* comp_match_list and bind *)
-   admit.
- - rewrite denote_comp_equation_5. (* comp_split and bind *)
-   admit.
- - rewrite denote_comp_equation_6. constructor. admit. split.
-   + intros.
-     assert (Hf : exists f, comp_equiv_rutt (MR := MR) (denote_value vf hyps) (ret f)).
-     admit.
-     destruct Hf as [f Hf]. specialize (H _ _ H1 _ _ Hf).
-     assert (Harg : exists arg, comp_equiv_rutt (MR := MR) (denote_value varg hyps) (ret arg)).
-     admit.
-     destruct Harg as [arg Harg].
-     specialize (H0 _ _ H1 _ _ Harg).
-     (* here is a situation where the amount of steps needs to decrease,
-        rewrite the approx_comp
-      *)
-     simp approx_val in H.
-
-   (* comp_app and bind *)
-   admit.
- - rewrite denote_comp_equation_7. (* comp_call and bind *)
-   admit.
- - rewrite denote_comp_equation_8. (* comp_mfix and interp_mrec *)
-   apply H0 in H1 as Hc. inversion Hc. subst. destruct H3 as [Hc1 Hc2].
-   apply H in H1 as Hbodies. 
-   (* I think this is showing I have the wrong bodies logical relation,
-      that idea I had that had something to do with bodies steps c
-      either to a ret or to an inr, then we need extra reasoning to 
-      bring the small step up to speed and the denotation
-    *) admit.
- - rewrite denote_comp_equation_9. apply H in H0 as Hc.
-   inversion Hc. subst. destruct H2 as [Hc1 Hc2].
-   constructor. admit.
-   split.
-   + intros. 
-     (* H1 can tell us everything about denote_comp c then we apply Hc1 to that info
-        then we know how c steps
-      *) admit.
-   + intros.
-     (* similar thing going on *) admit.
- - rewrite denote_comp_equation_10. apply H in H0 as Hc.
-   inversion Hc. subst. destruct H2 as [Hc1 Hc2].
-   (* morally similar to the previous *)
-   admit.
- - (* these cases are too broken to bother with right now *) admit.
- - admit. *) *)
-Admitted.
-
-Lemma adequacy : forall (c : comp Nat [] []) (n : nat),
+Lemma adequacy_aux : forall (c : comp Nat [] []) (n : nat),
     comp_equiv (denote_comp c) (denote_value (val_const n)) ->
     eval_rel c (val_const n).
 Proof.
-  destruct (fundamental_theorem_adequacy 2) as [Had _].
-  intros c n Hc.
-  specialize (Had Nat [] [] c tt tt (closing_subst_approx_nil 2)).
-  inversion Had. subst. clear Had. assert (2 > 0). auto. specialize (H H0) as [Hret _]. 
-  specialize (Hc tt tt I). apply Hret in Hc. clear - Hc. destruct Hc as [m [Hm1 Hm2]]. 
-  cbn in *. red in m. dependent destruction m; try inversion x. simp approx_val in Hm2.
-  subst. simp close_comp in Hm1. rename n0 into n. dependent induction Hm1.
-  - eapply eval_rel_step; eauto.
-  - eapply eval_rel_val; auto.
+  destruct fundamental_theorem_adequacy_mutind as [Had _].
+  intros. 
+  specialize (Had _ _ _ c). red in Had. red in H.
+  specialize (H tt tt I). simp denote_comp in H.
+  apply rutt_ret_eutt in H. simp types_equiv in H.
+  apply eutt_ret_multi_step in H as [j Hj].
+  specialize (Had (S j) tt tt (closing_subst_approx_nil _)).
+  inversion Had. subst.
+  assert (Hj' : j < S j). lia. 
+  specialize (H j Hj'). destruct H as [Hret _].
+  specialize (Hret n Hj). destruct Hret as [n' [Heval Happrox]].
+  assert (Hj'' : S j - j = 1). lia. rewrite Hj'' in Happrox.
+  red in n'. dependent destruction n'; try inversion x.
+  rewrite approx_val_equation_2 in Happrox. subst n0.
+  simp close_comp in Heval. apply eval_rel_stuck_eval_rel.
+  auto.
 Qed.
+
+Lemma adequacy t Γ MR (c1 c2 : comp t Γ MR) : 
+  comp_equiv (denote_comp c1) (denote_comp c2) ->
+  context_equiv c1 c2.
+Proof.
+  intros Hden C n.
+  assert (Hden' : comp_equiv 
+                    (denote_comp (subst_comp_context C c1))
+                    (denote_comp (subst_comp_context C c2))).
+  eapply subst_comp_context_proper; eauto.
+  remember (subst_comp_context C c1) as c1'.
+  remember (subst_comp_context C c2) as c2'. clear Heqc1' Heqc2' Hden c1 c2.
+  specialize (Hden' tt tt I).
+  split; intros Hstep; apply adequacy_aux.
+  - red. intros [] [] _. etransitivity. symmetry. eauto. eapply eval_stable. auto.
+  - red. intros [] [] _. etransitivity. eauto. eapply eval_stable; auto.
+Qed.
+(* Print Assumptions adequacy. close_comp_open2 *) 
+
