theories/AlmostStlc/EnTreeStep.v
@@ -1,3 +1,4 @@
+
 Require Export TypedVar.
 Require Export SyntaxSeq.
 Require Export SmallStepSeq.
@@ -18,7 +19,6 @@ Require Export CallMrecFacts.
 Require Export SemanticsFactsSeq2.
 Require Import Lia.
 Require Import ITree.Basics.HeterogeneousRelations.
-
 Require Import Coq.Classes.Morphisms.
 
 Local Open Scope entree_scope.
@@ -63,6 +63,18 @@ Proof.
   destruct H0. rewrite H0, tau_eutt. auto.
 Qed.
 
+Lemma multi_step_eq_itree_r {E R} `{EncodedType E} n (t1 t2 t3 : entree E R) :
+  multi_step n t1 t2 -> multi_step n t1 t3 -> t2 ≅ t3.
+Proof.
+  revert t1 t2 t3. induction n.
+  - intros. dependent destruction H0. rewrite H0 in H1. dependent destruction H1.
+    auto.
+  - intros. dependent destruction H0.
+    dependent destruction H1. dependent destruction H2.
+    dependent destruction H3. rewrite H1 in H3.
+    apply eqit_inv_Tau in H3. rewrite <- H3 in H2. eauto.
+Qed.
+
 Lemma eutt_ret_multi_step {E R} `{EncodedType E} (t : entree E R) (r : R) :
   t ≈ ret r -> exists n, multi_step n t (ret r).
 Proof.
@@ -88,6 +100,19 @@ Ltac remember_eq_itree t1 n :=
   let H1 := fresh in
   let H2 := fresh "Heq" in
   remember t1 as n eqn : H1; assert (H2 : t1 ≅ n); try (subst; reflexivity); clear H1.
+
+Lemma multi_step_bind E R1 R2 `{EncodedType E} (t t': entree E R1) (k : R1 -> entree E R2) n :
+  multi_step n t t' ->
+  multi_step n (bind t k) (bind t' k).
+Proof.
+  generalize dependent t. generalize dependent t'. revert k.
+  induction n.
+  - intros. dependent destruction H0. rewrite H0.
+    constructor. reflexivity.
+  - intros. dependent destruction H0. dependent destruction H1.
+    rewrite H1. setoid_rewrite bind_tau. econstructor. eauto. constructor.
+    reflexivity.
+Qed.
 
 Lemma multi_step_ret_bind_inv E R1 R2 `{EncodedType E} (t : entree E R1) (k : R1 -> entree E R2) s n : 
       multi_step n (x <- t;; k x) (ret s) -> 
@@ -144,4 +169,458 @@ Proof.
         econstructor; eauto. constructor. auto.
     + rewrite Hek in Heq. setoid_rewrite bind_vis in Heq.
       pinversion Heq. inversion CHECK.
+Qed.
+
+Lemma multi_step_mapE_inv_ret D1 D2 R `{EncodedType D1} `{EncodedType D2}
+      (h : handler D1 D2) t (r : R) j : 
+  valid_handler h ->
+  multi_step j (mapE h t) (ret r) ->
+  multi_step j t (ret r).
+Proof.
+  intros H1 H2. remember (mapE h t) as x.
+  assert (x ≅ mapE h t). subst. reflexivity. clear Heqx.
+  remember (ret r) as y.
+  assert (y ≅ ret r). subst. reflexivity. clear Heqy.
+  generalize dependent y. generalize dependent x. generalize dependent t.
+  induction j.
+  - intros. rewrite H3, H4 in H2. constructor.  dependent destruction H2.
+    destruct (eq_itree_case t) as [[r' Hr] | [[t' Ht'] | [e' [k' Hek]] ]].
+    + setoid_rewrite Hr in H2. setoid_rewrite mapE_ret in H2.
+      apply eqit_Ret_inv in H2.
+      subst. auto.
+    + rewrite Ht', mapE_tau in H2. pinversion H2. inversion CHECK.
+    + rewrite Hek, mapE_vis in H2. destruct (h e'). pinversion H2.
+  - intros. rewrite H3, H4 in H2. clear H3 H4. dependent destruction H2.
+    destruct (eq_itree_case t) as [[r' Hr] | [[t' Ht'] | [e' [k' Hek]] ]].
+    + rewrite Hr in H3. setoid_rewrite mapE_ret in H3.
+      dependent destruction H3. pinversion H3. inversion CHECK.
+    + rewrite Ht', mapE_tau in H3. dependent destruction H3.
+      apply eqit_inv_Tau in H3. econstructor; eauto.
+      eapply IHj with (t := t'); eauto. symmetry. auto.
+      reflexivity. constructor. auto.
+    + rewrite Hek, mapE_vis in H3. destruct (h e').
+      dependent destruction H3. pinversion H3. inversion CHECK.
+Qed.
+
+Lemma multi_step_mapE_vis D1 D2 R `{EncodedType D1} `{EncodedType D2}
+      (h : handler D1 D2) t e (k : _ -> entree D1 R) j :
+  valid_handler h ->
+  multi_step j t (Vis e k) ->
+  multi_step j (mapE h t) (let 'd' && f := h e in Vis d' (fun x : encodes d' => mapE h (k (f x)))).
+Proof.
+  intros.
+  remember (Vis e k) as y.
+  assert (y ≅ Vis e k). subst. reflexivity.
+  clear Heqy.
+  generalize dependent y. generalize dependent t. generalize dependent e.
+  induction j.
+  - intros. dependent destruction H2. rewrite H2, H3.
+    constructor. rewrite mapE_vis. reflexivity.
+  - intros. dependent destruction H2. dependent destruction H3.
+    rewrite H3, mapE_tau. econstructor. eauto.
+    constructor. reflexivity.
+Qed.
+
+Lemma multi_step_mapE_inv_vis D1 D2 R `{EncodedType D1} `{EncodedType D2}
+      (h : handler D1 D2) t e (k : _ -> entree D1 R) j : 
+  valid_handler h ->
+  multi_step j (mapE h t) (let 'd' && f := h e in Vis d' (fun x : encodes d' => mapE h (k (f x)))) ->
+  exists e' k', multi_step j t (Vis e' k').
+Proof.
+  intros H1 H2. remember (mapE h t) as x.
+  assert (x ≅ mapE h t). subst. reflexivity. clear Heqx.
+  remember ((let 'd' && f := h e in Vis d' (fun x : encodes d' => mapE h (k (f x))))) as y.
+  assert (y ≅ (let 'd' && f := h e in Vis d' (fun x : encodes d' => mapE h (k (f x))))).
+  subst. reflexivity. clear Heqy. generalize dependent x. generalize dependent y.
+  generalize dependent e.
+  generalize dependent t. induction j.
+  - intros. rewrite H3, H4 in H2. dependent destruction H2. clear H3 H4.
+    destruct (h e) as [d g] eqn : Heq.
+    destruct (eq_itree_case t) as [[r' Hr] | [[t' Ht'] | [e' [k' Hek]] ]].
+    + setoid_rewrite Hr in H2. setoid_rewrite mapE_ret in H2.
+      pinversion H2.
+    + rewrite Ht', mapE_tau in H2. pinversion H2. inversion CHECK.
+    + rewrite Hek, mapE_vis in H2. destruct (h e') eqn : Heq'.
+      assert (x0 = d).
+      pinversion H2. auto. subst. 
+      eexists. eexists. constructor. eauto.
+  - intros. rewrite H3, H4 in H2. clear H3 H4.
+    destruct (h e) as [d g] eqn : Heq.
+    destruct (eq_itree_case t) as [[r' Hr] | [[t' Ht'] | [e' [k' Hek]] ]].
+    + setoid_rewrite Hr in H2. setoid_rewrite mapE_ret in H2.
+      dependent destruction H2. dependent destruction H3.
+      pinversion H3. inversion CHECK.
+    + rewrite Ht', mapE_tau in H2. dependent destruction H2.
+      dependent destruction H3. apply eqit_inv_Tau in H3. symmetry in H3.
+      eapply IHj with (e := e) in H2; eauto.
+      * setoid_rewrite Ht'. destruct H2 as [e' [k' Hek']].
+        exists e', k'. econstructor; eauto. constructor. reflexivity.
+      * rewrite Heq. reflexivity.
+    + rewrite Hek in H2.
+      dependent destruction H2.
+      dependent destruction H3.
+      clear - H3. rewrite mapE_vis in H3.
+      destruct (h e'). pinversion H3. inversion CHECK.
+Qed.
+
+Lemma multi_step_mapE_inv_vis' D1 D2 R `{EncodedType D1} `{EncodedType D2}
+      (h : handler D1 D2) t e e' (k : _ -> entree D1 R) k' j : 
+  valid_handler h ->
+  multi_step j (mapE h t) (let 'd' && f := h e in Vis d' (fun x : encodes d' => mapE h (k (f x)))) ->
+  multi_step j t (Vis e' k') ->
+  projT1 (h e) = projT1 (h e').
+Proof.
+  intros. apply multi_step_eutt in H2.
+  apply multi_step_eutt in H3.
+  rewrite H3 in H2. rewrite mapE_vis in H2.
+  destruct (h e). destruct (h e'). cbn.
+  pinversion H2. auto.
+Qed.
+
+Lemma JMeq_mapE_aux:
+  forall A B C (MR1 MR2 : mfix_ctx)
+    (h : handler (denote_mrec_ctx (denote_mfix_ctx MR1)) (denote_mrec_ctx (denote_mfix_ctx MR2)))
+    (e' : denote_mrec_ctx (denote_mfix_ctx MR1)) (d :A -> B)
+    (e0 : C -> A) (k' : A -> entree (denote_mrec_ctx (denote_mfix_ctx MR1)) B)
+    (a : A),
+    valid_handler h ->
+    (forall x : C, mapE h (k' (e0 x)) ≅ Ret (d (e0 x))) ->
+    A = B -> d ~= (@id B) -> A = C -> e0 ~= (@id A) -> eqit eq false false (k' a) (Ret (d a)).
+Proof.
+  intros. subst. subst. unfold id in *.
+  specialize (H0 a).
+  destruct (eq_itree_case (k' a)) as [[r' Hr] | [[t' Ht'] | [e'' [k'' Hek]] ]].
+  - setoid_rewrite Hr in H0. setoid_rewrite mapE_ret in H0. apply eqit_Ret_inv in H0.
+    subst. auto.
+  - rewrite Ht', mapE_tau in H0. pinversion H0. inversion CHECK.
+  - rewrite Hek, mapE_vis in H0. destruct (h e''). pinversion H0.
+Qed.
+
+Lemma mapE_perm_handler_call_term_aux':
+  forall (t2 : vtype) (MR1 MR2 : mfix_ctx) (t0 : vtype) 
+    (R : call_frame) (yR : var R MR2) (x : var (t0, t2) R) (r1 r2 : denote_type t0)
+    h (vf : forall R, var R MR1 -> var R MR2) t,
+    var_map_handler_rel h vf ->
+    valid_handler h ->
+    (mapE h t) ≅ (call_term x yR r1) ->
+    exists xR, t ≅ call_term x xR r1 /\ vf _ xR = yR.
+Proof.
+  intros. unfold call_term in *.
+  destruct (call_mrec x yR r1) eqn : Heq1. setoid_rewrite bind_trigger in H1.
+  destruct (eq_itree_case t) as [[r' Hr] | [[t' Ht'] | [e' [k' Hek]] ]].
+  rewrite Hr in H1. setoid_rewrite mapE_ret in H1. pinversion H1.
+  rewrite Ht', mapE_tau in H1. pinversion H1. inversion CHECK.
+  setoid_rewrite Hek. rewrite Hek, mapE_vis in H1.
+  destruct (h e') eqn : Heq2. assert (x1 = x0). pinversion H1. auto.
+  subst.
+  specialize (call_extract _ (e')) as [R2 [xR [tin' [tout' [y [vvin' Hvvin']]]] ]].
+
+  red in H.
+  destruct (call_mrec y xR vvin') eqn : Heq3. cbn in Hvvin'. subst.
+  eapply H in Heq2 as ?; eauto.
+  assert (projT1 (call_mrec y (vf R2 xR) vvin') = projT1 (call_mrec x yR r1)). subst.
+  rewrite Heq1. auto.
+  eapply call_term_bind_inv_aux1 in H3 as ?. apply var_eq_surj in H4 as ?. subst.
+  apply var_eq_eq in H4. subst. exists xR.
+  eapply call_term_bind_inv_aux2 in H3 as ?. destruct H2.
+  apply var_eq_surj in v as ?. injection X. intros. subst. subst.
+  apply var_eq_eq in v. subst. rewrite Heq3. split; auto.
+  setoid_rewrite bind_trigger. apply eqit_Vis. intros.
+  specialize (H0 e') as H'. destruct H'. rewrite Heq2 in H4. cbn in H4.
+  clear H3 X.
+  specialize (call_mrec_encodes _ _ _ _ x xR vvin') as Henc1.
+  specialize (call_mrec_cont _ _ _ _ x xR vvin') as Henc2.
+  rewrite Heq3 in Henc1, Henc2.
+  rewrite Heq2 in H2. cbn in H2.
+  eapply JMeq_mapE_aux with (e0 := e); eauto.
+  intros. eapply eqit_Vis_inv in H1. rewrite H1. apply eqit_Ret.
+  symmetry. 
+  specialize (call_mrec_encodes _ _ _ _ x (vf _ xR) vvin') as Henc3.
+  specialize (call_mrec_cont _ _ _ _ x (vf _ xR) vvin') as Henc4.
+  rewrite Heq1 in Henc3, Henc4.
+  eapply JMeq_comp'; eauto.
+Qed.
+
+Lemma mapE_call_term_inv:
+  forall (tin tout : vtype) (R : call_frame) (MR1 MR2 : mfix_ctx) (xR : var R MR1) (vvin : denote_type tin)
+    (h : handler (denote_mrec_ctx (denote_mfix_ctx MR1)) (denote_mrec_ctx (denote_mfix_ctx MR2)))
+    (vf : forall R0 : call_frame, var R0 MR1 -> var R0 MR2)
+    (t : entree (denote_mrec_ctx (denote_mfix_ctx MR1)) (denote_type tout)) (x : var (tin, tout) R),
+    mapE h t ≅ call_term x (vf R xR) vvin ->
+    var_map_handler_rel h vf ->
+    valid_handler h -> (forall (R0 : call_frame) (x0 y : var R0 MR1), vf R0 x0 = vf R0 y -> x0 = y) -> t ≅ call_term x xR vvin.
+Proof.
+  intros tin tout R MR1 MR2 xR vvin h vf t x H Hhf Hh Hinj.
+  assert (mapE h t ≅ mapE h (call_term x xR vvin)).
+  erewrite mapE_perm_handler_call_term_aux; eauto. Locate mapE_perm_handler_call_term_aux. clear H.
+  rename H0 into Hmap.
+  unfold call_term in *. destruct (call_mrec x xR vvin) eqn : HeqxR.
+  setoid_rewrite bind_trigger. setoid_rewrite bind_trigger in Hmap.
+  setoid_rewrite mapE_vis in Hmap.
+  destruct (h x0) eqn : Heqx0. 
+  assert ( Vis x1 (fun x : encodes x1 => mapE h (ret (d (e x)))) ≅ Vis x1 (fun x => ret (d (e x)))).
+  apply eqit_Vis. intros. setoid_rewrite mapE_ret. reflexivity.
+  rewrite H in Hmap. clear H.
+  destruct (eq_itree_case t) as [[r' Hr] | [[t' Ht'] | [e' [k' Hek]] ]].
+  + rewrite Hr in Hmap. setoid_rewrite mapE_ret in Hmap. pinversion Hmap.
+  + rewrite Ht', mapE_tau in Hmap. pinversion Hmap. inversion CHECK.
+  + rewrite Hek, mapE_vis in Hmap.
+    destruct (h e') eqn : Heqe'. rewrite Hek.
+    assert (x1 = x2). pinversion  Hmap. auto.
+    subst x1.
+    assert (e' = x0). 
+    { 
+      eapply Hhf in HeqxR as ?; eauto. specialize (H Heqx0).
+      clear Hmap. subst x2.
+      specialize (call_extract _ (e')) as [R2 [yR [tin' [tout' [y [vvin' Hvvin']]]] ]].
+      subst e'. enough (projT1 (call_mrec y yR vvin') = projT1 (call_mrec x xR vvin)).
+      rewrite HeqxR in H; auto.
+      assert (projT1 (h (projT1 (call_mrec y yR vvin')) ) = projT1 (call_mrec y (vf _ yR) vvin')).
+      { red in Hhf. destruct (h (projT1 (call_mrec y yR vvin'))) eqn : ?.  erewrite Hhf; eauto.
+        Unshelve. 2 : apply (projT2 (call_mrec y yR vvin')). destruct (call_mrec y yR vvin').
+        auto.
+      } rewrite Heqe' in H. simpl in H.
+      eapply call_term_bind_inv_aux1 in H as ?. apply var_eq_surj in H0 as ?.
+      subst R2. apply var_eq_eq in H0.
+      assert (xR = yR). eapply Hinj. auto.
+      subst.
+      eapply call_term_bind_inv_aux2 in H as ?. destruct H1.
+      apply var_eq_surj in v as ?. injection X. intros. subst.
+      subst. apply var_eq_eq in v. subst. auto.
+    }
+    subst x0. apply eqit_Vis. intros.
+    assert (forall x, mapE h (k' (e0 x)) ≅ ret (d (e x))).
+    intros. eapply eqit_Vis_inv in Hmap; eauto.
+    specialize (call_mrec_encodes _ _ _ _ x xR vvin) as Henc1.
+    specialize (call_mrec_cont _ _ _ _ x xR vvin) as Henc2. rewrite HeqxR in Henc1, Henc2.
+    cbn in *. rewrite Heqx0 in Heqe'. inj_existT. subst.
+    specialize (Hh e') as H'. destruct H' as [Henc3 Henc4]. rewrite Heqx0 in Henc3, Henc4.
+    cbn in *. eapply JMeq_mapE_aux; eauto.
+Qed.
+
+
+
+Lemma multi_step_call_term_bind_ex tin tout R MR (xR : var R MR) (x : var (tin, tout) R) (vvin : denote_type tin)
+      S (k : _ -> mtree _ S) t n :
+  multi_step n t (bind (call_term x xR vvin) k) ->
+  exists t', t ≅ bind t' k /\ multi_step n t' (call_term x xR vvin).
+Proof.
+  revert k t. induction n.
+  - intros. dependent destruction H. exists (call_term x xR vvin).
+    split; auto. constructor. reflexivity.
+  - intros. dependent destruction H. dependent destruction H1. 
+    eapply IHn in H as [t' [Ht'1 Ht'2]]. exists (Tau t').
+    rewrite H0. setoid_rewrite bind_tau. split. pstep. constructor. auto.
+    econstructor. eauto. econstructor. pstep. constructor. left.
+    enough (t' ≅ t'); auto. reflexivity.
+Qed.
+
+Lemma id_eq_inv A B (Heq1 : A = B) (Heq2 : B = A) (a : A) :
+  id_eq Heq2 (id_eq Heq1 a) = a.
+Proof.
+  subst. dependent destruction Heq2. simp id_eq. auto.
+Qed.
+(* A : encodes x0
+   B : denote_type tout
+   C : encodes e'
+
+*)
+Lemma multi_step_mapE_call_term_bind_ex_aux1:
+  forall A B C (e : A -> C) (d : A -> B)
+    (H1' : C = B) (a : A), 
+    A = B -> e ~= (@id C) -> d ~= (@id B) ->
+    id_eq H1' (e a) = d a.
+Proof.
+  intros. subst. simp id_eq. auto.
+Qed.
+(*
+A : encodes x0
+B : encodes e'
+C : denote_type tout
+*)
+Lemma multi_step_mapE_call_term_bind_ex_aux2:
+  forall A B C (e : A -> B ) (x1 : C)
+    (Henc2 : C = A) (H1 : C = B), 
+    e ~= (@id B) -> 
+    e (id_eq Henc2 x1) = id_eq H1 x1.
+Proof.
+  intros. subst. simp id_eq. auto.
+Qed.
+          
+(*
+A : encodes x0
+B : denote_type tout
+*)
+
+Lemma multi_step_mapE_call_term_bind_ex_aux3:
+  forall A B (d  : A -> B)
+    (x1 : B) (Henc2 : B = A), 
+    d ~= (@id B) ->
+    d (id_eq Henc2 x1) = x1.
+Proof.
+  intros. subst. simp id_eq. auto.
+Qed.
+
+Lemma multi_step_mapE_call_term_bind_ex tin tout R MR1 MR2 yR (x : var (tin, tout) R) (vvin : denote_type tin)
+      S (k : _ -> mtree (denote_mfix_ctx MR2) S) (t : mtree (denote_mfix_ctx MR1) S) (h : handler _ _) 
+       (vf : forall R0, var R0 MR1 -> var R0 MR2) n :
+  var_map_handler_rel h vf -> valid_handler h ->
+  multi_step n (mapE h t) (bind (call_term x yR vvin) k) ->
+  exists (t' : mtree _ _) (k' : _ -> mtree _ _), 
+    t ≅ bind t' k' /\ multi_step n (mapE h t') (call_term x yR vvin) /\ (forall x, k x ≅ mapE h (k' x)).
+Proof.
+  revert k t. induction n.
+  - intros k t H H0 H2. subst. dependent destruction H2. 
+    destruct (eq_itree_case t) as [[r' Hr] | [[t' Ht'] | [e' [k' Hek]] ]].
+    + rewrite Hr in H2. setoid_rewrite mapE_ret in H2. unfold call_term in H2.
+      destruct (call_mrec x yR vvin). setoid_rewrite bind_trigger in H2.
+      setoid_rewrite bind_vis in H2. pinversion H2.
+    + exfalso. rewrite Ht', mapE_tau in H2. unfold call_term in H2.
+      destruct (call_mrec x yR vvin). setoid_rewrite bind_trigger in H2.
+      setoid_rewrite bind_vis in H2. pinversion H2. inversion CHECK.
+    + specialize (call_mrec_encodes _ _ _ _ x yR vvin) as Henc1.
+      (* need a function from denote_type tout to encode e'*)
+      rewrite Hek, mapE_vis in H2.
+      destruct (h e') eqn : Heqhe'. unfold call_term in H2.
+      destruct (call_mrec x yR vvin) eqn : Heqcall.
+      setoid_rewrite bind_trigger in H2. setoid_rewrite bind_vis in H2.
+      assert (x1 = x0). pinversion H2. auto.
+      subst. 
+      assert (denote_type tout = encodes e').
+      { red in H0. specialize (H0 e') as H1. destruct H1. rewrite Heqhe' in H1. cbn in H1.
+        rewrite H1. specialize (call_mrec_encodes _ _ _ _ x yR vvin) as Henc2.
+        rewrite Heqcall in Henc2. setoid_rewrite Henc2. auto.
+      } assert (H1' : encodes e' = denote_type tout). rewrite H1. auto.
+      exists (Vis e' (fun x => ret (id_eq H1' x))).
+      exists (fun x => k' (id_eq H1 x)).
+      split; [ | split].
+      * rewrite Hek. setoid_rewrite bind_vis. apply eqit_Vis. 
+        intros. setoid_rewrite bind_ret_l. rewrite id_eq_inv.
+        reflexivity.
+      * constructor. rewrite mapE_vis. rewrite Heqhe'.
+        unfold call_term. rewrite Heqcall. setoid_rewrite bind_trigger.
+        apply eqit_Vis. intros. rewrite mapE_ret. apply eqit_Ret.
+        specialize (call_mrec_encodes _ _ _ _ x yR vvin) as Henc2.
+        specialize (call_mrec_cont _ _ _ _ x yR vvin) as Henc3.
+        rewrite Heqcall in Henc2, Henc3. cbn in Henc2, Henc3.
+        specialize (H0 e') as ?. rewrite Heqhe' in H3. cbn in H3.
+        destruct H3.
+        eapply multi_step_mapE_call_term_bind_ex_aux1; eauto.
+      * intros. specialize (call_mrec_encodes _ _ _ _ x yR vvin) as Henc2.
+        rewrite Heqcall in Henc2. cbn in Henc2. symmetry in Henc2.
+        eapply eqit_Vis_inv with (a := id_eq Henc2 x1) in H2. symmetry.
+        assert (e (id_eq Henc2 x1) = id_eq H1 x1).
+        specialize (H0 e'). destruct H0. rewrite Heqhe' in H3. cbn in H3.
+        eapply multi_step_mapE_call_term_bind_ex_aux2; eauto.
+        assert (d (id_eq Henc2 x1) = x1).
+        eapply multi_step_mapE_call_term_bind_ex_aux3.
+        specialize (call_mrec_cont _ _ _ _ x yR vvin) as Henc3.
+        rewrite Heqcall in Henc3. auto.
+        rewrite H3, H4 in H2. rewrite H2. setoid_rewrite bind_ret_l. 
+        reflexivity.
+  - intros. dependent destruction H1. dependent destruction H3. 
+    destruct (eq_itree_case t) as [[r' Hr] | [[t' Ht'] | [e' [k' Hek]] ]].
+    + rewrite Hr in H2. setoid_rewrite mapE_ret in H2. pinversion H2. inversion CHECK.
+    + rewrite Ht', mapE_tau in H2. apply eqit_inv_Tau in H2. rewrite <- H2 in H1.
+      eapply IHn in H1; eauto. destruct H1 as [t'' [k'' [? [? ?]]]].
+      setoid_rewrite Ht'. exists (Tau t''), k''. setoid_rewrite bind_tau.
+      split. pstep. constructor. auto. split; auto. setoid_rewrite mapE_tau.
+      econstructor. eauto. constructor. reflexivity.
+    + rewrite Hek, mapE_vis in H2. destruct (h e'). pinversion H2. inversion CHECK.
+Qed.
+(*
+Lemma multi_step_mapE_call_term_inv tin tout R S MR1 MR2 (xR : var R MR1) (yR : var R MR2) (x : var (tin, tout) R) (vvin : denote_type tin) t (k : _ -> mtree _ S)
+      h (vf : forall R0, var R0 MR1 -> var R0 MR2) n : 
+  (forall R0 (x y: var R0 MR1), vf _ x = vf _ y -> x = y) ->
+  var_map_handler_rel h vf -> valid_handler h ->
+  vf R xR = yR ->
+  multi_step n (mapE h t) (bind (call_term x yR vvin) k) ->
+  exists k', multi_step n t (bind (call_term x xR vvin) k').
+*)
+
+(* this is hideous, may need to add a continuation to bind to
+   get that lemma by combining this with 
+   multi_step_vis_bind_inv
+   actually that does not give us what we want 
+
+   but I think what I do what is derivable from bind metatheory and this
+   gross lemma
+
+  t ->j bind call k -> exists t1 k,
+  t ≅ bind t1 k /\ t1 -> j call ?
+
+ *)
+(*
+Lemma 
+  mapE h t ≅ call_term x yR vvin ->
+  exists xR, t ≅ call_term 
+*)
+Lemma multi_step_mapE_call_term_inv tin tout R MR1 MR2 (yR : var R MR2) (x : var (tin, tout) R) (vvin : denote_type tin) t 
+      h (vf : forall R0, var R0 MR1 -> var R0 MR2) n : 
+  (forall R0 (x y: var R0 MR1), vf _ x = vf _ y -> x = y) ->
+  var_map_handler_rel h vf -> valid_handler h ->
+  multi_step n (mapE h t) (call_term x yR vvin) ->
+  exists xR, multi_step n t (call_term x xR vvin) /\ vf R xR = yR.
+Proof.
+  intros Hinj Hhf Hh Hstep. subst.
+  remember (mapE h t) as xt.
+  assert (xt ≅ mapE h t). subst. reflexivity.
+  remember ((call_term x yR vvin)) as yt.
+  assert (yt ≅ (call_term x yR vvin)). subst. reflexivity.
+  clear Heqyt Heqxt.
+  generalize dependent x. generalize dependent t.
+  generalize dependent xt. generalize dependent yt.
+  induction n.
+  - intros. dependent destruction Hstep. rewrite H1, H0 in H.
+    clear H0 H1. eapply mapE_perm_handler_call_term_aux' in H as ?; eauto.
+    destruct H0 as [xR [H1 H2]]. subst. exists xR. split; auto.
+    constructor. auto.
+  - intros. dependent destruction Hstep.
+    dependent destruction H. rewrite H in H0.
+    destruct (eq_itree_case t) as [[r' Hr] | [[t' Ht'] | [e' [k' Hek]] ]].
+    + rewrite Hr in H0. setoid_rewrite mapE_ret in H0. pinversion H0. inversion CHECK.
+    + rewrite Ht', mapE_tau in H0. apply eqit_inv_Tau in H0. eapply IHn in Hstep; eauto.
+      destruct Hstep as [xR [Hstep HxR]]. subst. exists xR.
+      split; auto. rewrite Ht'. econstructor. eauto. constructor. reflexivity.
+    + rewrite Hek, mapE_vis in H0. destruct (h e'). pinversion H0. inversion CHECK.
+Qed.
+
+Lemma multi_step_mapE_call_term_inv' tin tout R S MR1 MR2 (yR : var R MR2) (x : var (tin, tout) R) (vvin : denote_type tin) t (k : _ -> mtree _ S)
+      h (vf : forall R0, var R0 MR1 -> var R0 MR2) n : 
+  (forall R0 (x y: var R0 MR1), vf _ x = vf _ y -> x = y) ->
+  var_map_handler_rel h vf -> valid_handler h ->
+  multi_step n (mapE h t) (bind (call_term x yR vvin) k) ->
+  exists xR k', multi_step n t (bind (call_term x xR vvin) k') /\ vf R xR = yR /\ (forall x, k x ≅ mapE h (k' x)).
+Proof.
+  intros Hinj Hvf Hh Hstep. eapply multi_step_mapE_call_term_bind_ex in Hstep as Hstep'; eauto.
+  destruct Hstep' as [t' [k' [Ht'1 [Ht'2 Ht'3]]]].
+  eapply multi_step_mapE_call_term_inv in Ht'2; eauto. destruct Ht'2 as [xR [Ht'4 HxR]].
+  subst. exists xR. exists k'. split; [ | split]; eauto.
+  rewrite Ht'1. apply multi_step_bind; eauto.
+Qed.
+
+Lemma multi_step_perm_inv S tin tout R MR1 MR2 (Hperm : perm MR1 MR2) 
+      (yR : var R MR2) (x : var (tin, tout) R) (vvin : denote_type tin) t 
+      (k : _ -> mtree _ S) n : 
+  multi_step n (map_perm _ _ (perm_denote Hperm)  t) (bind (call_term x yR vvin) k) ->
+  exists xR k', multi_step n t (bind (call_term x xR vvin) k') /\ perm_var xR Hperm = yR /\ 
+             (forall x, k x ≅ map_perm  _ _ (perm_denote Hperm) (k' x)).
+Proof.
+  intros. eapply multi_step_mapE_call_term_inv' in H; try eapply perm_var_map_handler_rel with (Hperm := Hperm); try apply valid_perm_handler; 
+    try apply perm_var_inj; eauto.
+Qed.
+
+
+
+Lemma multi_step_lift_inv S tin tout R MR1 MR2
+      (yR : var R (MR1 ++ MR2)) (x : var (tin, tout) R) (vvin : denote_type tin) t 
+   (k : _ -> mtree _ S) n : 
+  multi_step n (mapE (lift_handler _) t) (bind (call_term x yR vvin) k) ->
+  exists xR k', multi_step n t (bind (call_term x xR vvin) k') /\ 
+             weaken_var_l _ _ _ xR = yR /\
+             (forall x, k x ≅ mapE (lift_handler _) (k' x)).
+Proof.
+  intros. eapply multi_step_mapE_call_term_inv' in H;
+    try eapply lift_handler_rel; try apply valid_lift_handler; eauto.
+  intros. eapply weaken_var_l_inj; eauto.
 Qed.
